src/riscv/Platform/AtomicMinimal.v
@@ -63,6 +63,7 @@ Section Riscv.
       Primitives.is_initial_register_value := eq (word.of_Z 0);
       Primitives.nonmem_load n kind addr _ _ := False;
       Primitives.nonmem_store n kind addr v _ _ := False;
+      Primitives.valid_machine mach := True;
     }.
 
 End Riscv.
